\documentclass{article}
\usepackage[utf8]{inputenc}
\usepackage{amsmath}
\newcommand{\ket}[1]{\left |{#1}\right \rangle}
\newcommand{\bra}[1]{\left \langle {#1}\right |}
\newcommand{\D}[3]{D^{#1}_{{#2}{#3}}}%(\phi,\theta,\chi)}
\newcommand{\redrotmat}[3]{d^{#1}_{{#2}{#3}}(\theta)}
\newcommand{\wigner}[6]{\begin{pmatrix}{#1}&{#2}&{#3}\\{#4}&{#5}&{#6}\end{pmatrix}}
\begin{document}

\begin{equation*}
\ket{JKM}=(-1)^{M-K}\left[\frac{2J+1}{8\pi^2}\right]^{\frac{1}{2}}\D{J}{-M}{-K}
\end{equation*}
\begin{equation*}
\bra{JKM}=\left[\frac{2J+1}{8\pi^2}\right]^{\frac{1}{2}}\D{J}{M}{K}
\end{equation*}
\begin{align*}
  \int\D{J_3}{M_3'}{M_3}\D{J_2}{M_2'}{M_2}\D{J_1}{M_1'}{M_1}d\Omega=\\8\pi^2 \wigner{J_1}{J_2}{J_3}{M_1}{M_2}{M_3}\wigner{J_1}{J_2}{J_3}{K_1}{K_2}{K_3}
\end{align*}
\begin{equation*}
  \begin{bmatrix}
    X\\
    Y\\
    Z\\
  \end{bmatrix}=
  \begin{bmatrix}
    c\phi~c\theta~c\chi-s\phi~s\chi &-c\phi~c\theta~s\chi-s\phi~c\chi & c\phi~s\theta\\
    s\phi~c\theta~c\chi+c\phi~s\chi &-s\phi~c\theta~s\chi+c\phi~c\chi & s\phi~s\theta\\ 
    -s\theta~c\chi & s\theta~s\chi & c\theta\\
  \end{bmatrix}
  \begin{bmatrix}
    x\\
    y\\
    z\\
  \end{bmatrix}
\end{equation*}
Choose the external static field to be along the lab fixed Z axis. The dipole moment component along the Z axis is:
\begin{equation*}
  \mu_Z=-\sin(\theta)\cos(\chi)\mu_{Zx}+\sin(\theta)\sin(\chi)\mu_{Zy}+\cos(\theta)\mu_{Zz}
\end{equation*}
The static field Hamiltonian is:
\begin{equation*}
  H_s=-\mathbf{\mu}\cdot\mathbf{E}=-E\cdot \left[-\sin(\theta)\cos(\chi)\mu_{Zx}+\sin(\theta)\sin(\chi)\mu_{Zy}+\cos(\theta)\mu_{Zz}\right]
\end{equation*}
All the trigonometric functions can be expressed as D matrixes using table 3.1 page 89 in Zare

\begin{equation*}
  \D{J}{M'}{M}=e^{-i\phi M'}\redrotmat{J}{M'}{M}e^{-i\chi M}
\end{equation*}
\begin{equation*}
  cos(\theta)=\D{1}{0}{0}
\end{equation*}
\begin{equation*}
  \sin(\theta)\cos(\chi)= \frac{1}{\sqrt{2}}[\D{1}{0}{1}-\D{1}{0}{-1}]
\end{equation*}
\begin{equation*}
  \sin(\theta)\sin(\chi)= \frac{1}{\sqrt{2}}[\D{1}{0}{-1}+\D{1}{0}{1}]
\end{equation*}
Choose the laser electric field to be polarized along the Z axis. 
\begin{equation*}
  H_{laser}=-\frac{1}{4}\epsilon(t)^2\left[\sin^2\theta(\alpha_{xx}\cos^2(\chi)+\alpha_{yy}\sin^2(\chi))+\cos^2(\theta)\alpha_{zz}\right]
\end{equation*}

\begin{equation*}
  \sin^2(\theta)\cos^2(\chi) = \sqrt{\frac{1}{6}}(\D{2}{0}{2}+\D{2}{0}{-2})+\frac{1}{3}(1-\D{2}{0}{0})
\end{equation*}

\begin{equation*}
  \sin^2(\theta)\sin^2(\chi) = -\sqrt{\frac{1}{6}}(\D{2}{0}{-2}+\D{2}{0}{2})+\frac{1}{3}(1-\D{2}{0}{0})
\end{equation*}

\begin{equation*}
  \cos^2(\theta)=\frac{1}{3}+\frac{2}{3}\D{2}{0}{0}
\end{equation*}
Inserting in the Hamiltonian:

\begin{align*}
  H_{laser}-\frac{1}{4}\epsilon^2\Bigg[\sqrt{\frac{1}{6}}[\D{2}{0}{2}+\D{2}{0}{-2}][\alpha_{xx}-\alpha_{yy}]\\ +\frac{1}{3}(\alpha_{xx}+\alpha_{yy}+\alpha_{zz})+\frac{1}{3}\D{2}{0}{0}(2\alpha_{zz}-\alpha_{yy}-\alpha_{zz})\Bigg]
\end{align*}
We need to calculate
\begin{equation*}
  \int \D{J'}{M'}{K'}\D{2}{0}{2}\D{J}{M}{K}d\Omega=8\pi^2\wigner{J}{2}{J'}{-M}{0}{M'}\wigner{J}{2}{J'}{-K}{2}{K'}
\end{equation*}
\begin{equation*}
  \int \D{J'}{M'}{K'}\D{2}{0}{-2}\D{J}{M}{K}d\Omega=8\pi^2\wigner{J}{2}{J'}{-M}{0}{M'}\wigner{J}{2}{J'}{-K}{-2}{K'}
\end{equation*}
\begin{equation*}
  \int \D{J'}{M'}{K'}\D{2}{0}{0}\D{J}{M}{K}d\Omega=8\pi^2\wigner{J}{2}{J'}{-M}{0}{M'}\wigner{J}{2}{J'}{-K}{0}{K'}
\end{equation*}
First all M matrix elements:
$J'=J$
\begin{equation*}
  \wigner{J}{2}{J}{-M}{0}{M}=(-1)^{J+M}2A_2(2J+3)[3M^2-J(J+1)]
\end{equation*}
$J'=J+1$
\begin{equation*}
  \wigner{J}{2}{J+1}{-M}{0}{M}=(-1)^{J+M+1}A_2(2J+4)2M[6(J-M+1)(J+M+1)]^{1/2}
\end{equation*}
$J'=J-1$
\begin{equation*}
  \wigner{J}{2}{J-1}{-M}{0}{M}=(-1)^{J+M}A_2(2J+2)2M[6(J+M)(J-M)]^{1/2}
\end{equation*}
$J'=J+2$
\begin{equation*}
  \wigner{J}{2}{J+2}{-M}{0}{M}=(-1)^{J+M}A_2(2J+5)[6(J-M+2)(J-M+1)(J+M+2)(J+M+1)]^{1/2}
\end{equation*}
$J'=J-2$
\begin{equation*}
  \wigner{J}{2}{J-2}{-M}{0}{M}=(-1)^{J+M}A_2(2J+1)[6(J+M)(J+M-1)(J-M)(J-M-1)]^{1/2}
\end{equation*}
\newpage
Then the K elements +2
 $J'=J$ $K'=K-2$
\begin{equation*}
  \wigner{J}{2}{J}{-K}{2}{K-2}=(-1)^{J+K}A_2(2J+3)[6(J-K+1)(J-K+2)(J+K-1)(J+K)]^{1/2}
\end{equation*}
$J'=J+1$
\begin{equation*}
  \wigner{J}{2}{J+1}{-K}{2}{K-2}=(-1)^{J+K+1}A_2(2J+4)[4(J-K+1)(J-K+2)(J-K+3)(J+K)]^{1/2}
\end{equation*}
$J'=J-1$
\begin{equation*}
  \wigner{J}{2}{J-1}{-K}{2}{K-2}=(-1)^{J+K+1}A_2(2J+2)[4(J+K-2)(J+K-1)(J+K)(J-K+1)]^{1/2}
\end{equation*}
$J'=J+2$
\begin{equation*}
  \wigner{J}{2}{J+2}{-K}{2}{K-2}=(-1)^{J+K}A_2(2J+5)[(J-K+1)(J-K+2)(J-K+3)(J-K+4)]^{1/2}
\end{equation*}
$J'=J-2$
\begin{equation*}
  \wigner{J}{2}{J-2}{-K}{2}{K-2}=(-1)^{J+K}A_2(2J+1)[(J+K-3)(J+K-2)(J+K-1)(J+K)]^{1/2}
\end{equation*}
Then the K elements -2
 $J'=J$ $K'=K-2$
\begin{equation*}
  \wigner{J}{2}{J}{-K}{-2}{K+2}=(-1)^{J+K}A_2(2J+3)[6(J+K+1)(J+K+2)(J-K-1)(J-K)]^{1/2}
\end{equation*}
$J'=J+1$
\begin{equation*}
  \wigner{J}{2}{J+1}{-K}{-2}{K+2}=(-1)^{J+K}A_2(2J+4)[4(J+K+1)(J+K+2)(J+K+3)(J-K)]^{1/2}
\end{equation*}
$J'=J-1$
\begin{equation*}
  \wigner{J}{2}{J-1}{-K}{-2}{K+2}=(-1)^{J+K}A_2(2J+2)[4(J-K-2)(J-K-1)(J-K)(J+K+1)]^{1/2}
\end{equation*}
$J'=J+2$
\begin{equation*}
  \wigner{J}{2}{J+2}{-K}{-2}{K+2}=(-1)^{J+K}A_2(2J+5)[(J+K+1)(J+K+2)(J+K+3)(J+K+4)]^{1/2}
\end{equation*}
$J'=J-2$
\begin{equation*}
  \wigner{J}{2}{J-2}{-K}{-2}{K+2}=(-1)^{J+K}A_2(2J+1)[(J-K-3)(J-K-2)(J-K-1)(J-K)]^{1/2}
\end{equation*}
\section{D's}
\subsection{J'=J}
$K'=K$
\begin{align*}
\wigner{J}{2}{J}{-M}{0}{M}\wigner{J}{2}{J}{-K}{0}{K}=\\4(-1)^{J+M}A_2(2J+3)[3M^2-J(J+1)]*\\(-1)^{J+K}A_2(2J+3)[3K^2-J(J+1)]
\end{align*}
$K'=K-2$
\begin{align*}
\wigner{J}{2}{J}{-M}{0}{M}\wigner{J}{2}{J}{-K}{2}{K-2}=\\(-1)^{J+M}A_2(2J+3)[3M^2-J(J+1)]*\\(-1)^{J+K}A_2(2J+3)[6(J-K+1)(J-K+2)(J+K-1)(J+K)]^{1/2}
\end{align*}
$K'=K+2$
\begin{align*}
\wigner{J}{2}{J}{-M}{0}{M}\wigner{J}{2}{J}{-K}{-2}{K+2}=\\(-1)^{J+M}A_2(2J+3)[3M^2-J(J+1)]*\\(-1)^{J+K}A_2(2J+3)[6(J+K+1)(J+K+2)(J-K-1)(J-K)]^{1/2}
\end{align*}
\newpage
\subsection{J'=J+1}
$K'=K$
\begin{align*}
\wigner{J}{2}{J+1}{-M}{0}{M}\wigner{J}{2}{J+1}{-K}{0}{K}=\\(-1)^{J+M+1}A_2(2J+4)2M[6(J-M+1)(J+M+1)]^{1/2}*\\(-1)^{J+K+1}A_2(2J+4)2M[6(J-K+1)(J+K+1)]^{1/2}
\end{align*}
$K'=K-2$
\begin{align*}
\wigner{J}{2}{J+1}{-M}{0}{M}\wigner{J}{2}{J+1}{-K}{2}{K-2}=\\(-1)^{J+M+1}A_2(2J+4)2M[6(J-M+1)(J+M+1)]^{1/2}*\\(-1)^{J+K+1}A_2(2J+4)[4(J-K+1)(J-K+2)(J-K+3)(J+K)]^{1/2}
\end{align*}
$K'=K+2$
\begin{align*}
\wigner{J}{2}{J+1}{-M}{0}{M}\wigner{J}{2}{J+1}{-K}{-2}{K+2}=\\(-1)^{J+M+1}A_2(2J+4)2M[6(J-M+1)(J+M+1)]^{1/2}*\\(-1)^{J+K}A_2(2J+4)[4(J+K+1)(J+K+2)(J+K+3)(J-K)]^{1/2}
\end{align*}
\subsection{J'=J-1}
$K'=K$
\begin{align*}
\wigner{J}{2}{J-1}{-M}{0}{M}\wigner{J}{2}{J-1}{-K}{0}{K}=\\(-1)^{J+M}A_2(2J+2)2M[6(J+M)(J-M)]^{1/2}*\\(-1)^{J+K}A_2(2J+2)2K[6(J+K)(J-K)]^{1/2}
\end{align*}
$K'=K-2$
\begin{align*}
\wigner{J}{2}{J-1}{-M}{0}{M}\wigner{J}{2}{J-1}{-K}{2}{K-2}=\\(-1)^{J+M}A_2(2J+2)2M[6(J+M)(J-M)]^{1/2}*\\(-1)^{J+K+1}A_2(2J+2)[4(J+K-2)(J+K-1)(J+K)(J-K+1)]^{1/2}
\end{align*}
$K'=K+2$
\begin{align*}
\wigner{J}{2}{J-1}{-M}{0}{M}\wigner{J}{2}{J-1}{-K}{-2}{K+2}=\\(-1)^{J+M}A_2(2J+2)2M[6(J+M)(J-M)]^{1/2}*\\(-1)^{J+K}A_2(2J+2)[4(J-K-2)(J-K-1)(J-K)(J+K+1)]^{1/2}
\end{align*}
\newpage
\subsection{J'=J+2}
$K'=K$
\begin{align*}
\wigner{J}{2}{J+2}{-M}{0}{M}\wigner{J}{2}{J+2}{-K}{0}{K}=\\(-1)^{J+M}A_2(2J+5)[6(J-M+2)(J-M+1)(J+M+2)(J+M+1)]^{1/2}*\\(-1)^{J+K}A_2(2J+5)[6(J-K+2)(J-K+1)(J+K+2)(J+K+1)]^{1/2}
\end{align*}
$K'=K-2$
\begin{align*}
\wigner{J}{2}{J+2}{-M}{0}{M}\wigner{J}{2}{J+2}{-K}{2}{K-2}=\\(-1)^{J+M}A_2(2J+5)[6(J-M+2)(J-M+1)(J+M+2)(J+M+1)]^{1/2}*\\(-1)^{J+K}A_2(2J+5)[(J-K+1)(J-K+2)(J-K+3)(J-K+4)]^{1/2}
\end{align*}
$K'=K+2$
\begin{align*}
\wigner{J}{2}{J+2}{-M}{0}{M}\wigner{J}{2}{J+2}{-K}{-2}{K+2}=\\(-1)^{J+M}A_2(2J+5)[6(J-M+2)(J-M+1)(J+M+2)(J+M+1)]^{1/2}*\\(-1)^{J+K}A_2(2J+5)[(J+K+1)(J+K+2)(J+K+3)(J+K+4)]^{1/2}
\end{align*}
$K'=K$
\subsection{J'=J-2}
\begin{align*}
\wigner{J}{2}{J-2}{-M}{0}{M}\wigner{J}{2}{J-2}{-K}{0}{K}=\\(-1)^{J+M}A_2(2J+1)[6(J+M)(J+M-1)(J-M)(J-M-1)]^{1/2}*\\(-1)^{J+K}A_2(2J+1)[6(J+K)(J+K-1)(J-K)(J-K-1)]^{1/2}
\end{align*}
$K'=K-2$
\begin{align*}
\wigner{J}{2}{J-2}{-M}{0}{M}\wigner{J}{2}{J-2}{-K}{2}{K-2}=\\(-1)^{J+M}A_2(2J+1)[6(J+M)(J+M-1)(J-M)(J-M-1)]^{1/2}*\\(-1)^{J+K}A_2(2J+1)[(J+K-3)(J+K-2)(J+K-1)(J+K)]^{1/2}
\end{align*}
$K'=K+2$
\begin{align*}
\wigner{J}{2}{J-2}{-M}{0}{M}\wigner{J}{2}{J-2}{-K}{-2}{K+2}=\\(-1)^{J+M}A_2(2J+1)[6(J+M)(J+M-1)(J-M)(J-M-1)]^{1/2}*\\(-1)^{J+K}A_2(2J+1)[(J-K-3)(J-K-2)(J-K-1)(J-K)]^{1/2}
\end{align*}
\section{matrix elements}
\subsection{$J'=J$}

\begin{align*}
  \bra{JKM}H_{laser}\ket{JKM}=\\\bigg[-\frac{1}{4}\epsilon^2\bigg]\cdot\bigg[\frac{1}{3}[\alpha_{xx}+\alpha_{yy}+\alpha_{zz}]+\frac{4}{3}[2J+1]\cdot[2\alpha_{zz}-\alpha_{xx}-\alpha_{yy}]\cdot\\A_2(2J+3)^2[3M^2-J(J+1)]\cdot[3K^2-J(J+1)]\bigg]
\end{align*}
\begin{align*}
  \bra{JK\pm 2M}H_{laser}\ket{JKM}=-\frac{1}{4}\epsilon^2\cdot [2J+1] [\alpha_{xx}-\alpha_{yy}]\cdot A_2(2J+3)^2[3M^2-J(J+1)]\cdot\\ [6(J\pm K+1)(J \pm K+2)(J \mp K-1)(J \mp K)]^{1/2}
\end{align*}
\subsection{$J'=J+1$}
%\begin{align*}
 % \bra{J+1KM}H_{laser}\ket{JKM}=\\\bigg[-\frac{1}{4}\epsilon^2\bigg]\cdot \bigg[\frac{1}{3}[2\alpha_{zz}-\alpha_{xx}-\alpha_{yy}]\cdot\\(-1)^{J+M+1}A_2(2J+4)2M[6(J-M+1)(J+M+1)]^{1/2}\cdot\\(-1)^{J+K+1}A_2(2J+4)2M[6(J-K+1)(J+K+1)]^{1/2}\bigg]
%\end{align*}
\begin{align*}
  \bra{J+1KM}H_{laser}\ket{JKM}=\\\bigg[-\frac{1}{4}\epsilon^2\bigg]\cdot \bigg[ \sqrt{(2J+1)(2J+3)}\bigg] \bigg[\frac{1}{3}[2\alpha_{zz}-\alpha_{xx}-\alpha_{yy}]\cdot\\A_2(2J+4)^24MK [6(J-M+1)(J+M+1)]^{1/2}\cdot\\ [6(J-K+1)(J+K+1)]^{1/2}\bigg]
\end{align*}
%\begin{align*}
%  \bra{J+1K-2M}H_{laser}\ket{JKM}=-\frac{1}{4}\epsilon^2\cdot[\alpha_{xx}-\alpha_{yy}]\cdot\\(-1)^{J+M+1}A_2(2J+4)2M[6(J-M+1)(J+M+1)]^{1/2}\cdot\\(-1)^{J+K+1}A_2(2J+4)[4(J-K+1)(J-K+2)(J-K+3)(J+K)]^{1/2}
%\end{align*}
%\begin{align*}
%  \bra{J+1K+2M}H_{laser}\ket{JKM}=-\frac{1}{4}\epsilon^2\cdot[\alpha_{xx}-\alpha_{yy}]\cdot\\(-1)^{J+M+1}A_2(2J+4)2M[6(J-M+1)(J+M+1)]^{1/2}\cdot\\(-1)^{J+K}A_2(2J+4)[4(J+K+1)(J+K+2)(J+K+3)(J-K)]^{1/2}
%\end{align*}

\begin{align*}
  \bra{J+1K\pm2M}H_{laser}\ket{JKM}=\bigg[ \pm\frac{1}{4}\epsilon^2 \bigg] \cdot \bigg[ \sqrt{(2J+1)(2J+3)}\bigg] \cdot[\alpha_{xx}-\alpha_{yy}]\cdot\\A_2(2J+4)^22M[6(J-M+1)(J+M+1)]^{1/2}\cdot\\ [4(J\pm K+1)(J\pm K+2)(J\pm K+3)(J\mp K)]^{1/2}
\end{align*}
%\subsection{$J'=J-1$}
%\begin{align*}
%  \bra{J-1KM}H_{laser}\ket{JKM}=\\\bigg[-\frac{1}{4}\epsilon^2 \bigg] \cdot \bigg[ \sqrt{(2J+1)(2J-1)} \bigg] \bigg[\frac{1}{3}[2\alpha_{zz}-\alpha_{xx}-\alpha_{yy}]\cdot\\ A_2(2J+2)^24MK[6(J+M)(J-M)]^{1/2}\cdot \\ [6(J+K)(J-K)]^{1/2}
%\end{align*}
%\begin{align*}
%  \bra{J-1K-2M}H_{laser}\ket{JKM}=(-1)^{J+M}A_2(2J+2)2M[6(J+M)(J-M)]^{1/2}*\\(-1)^{J+K+1}A_2(2J+2)[4(J+K-2)(J+K-1)(J+K)(J-K+1)]^{1/2}
%\end{align*}
%\begin{align*}
%  \bra{J-1K+2M}H_{laser}\ket{JKM}=\\(-1)^{J+M}A_2(2J+2)2M[6(J+M)(J-M)]^{1/2}*\\(-1)^{J+K}A_2(2J+2)[4(J-K-2)(J-K-1)(J-K)(J+K+1)]^{1/2}
%\end{align*}
%\begin{align*}
%  \bra{J-1K\pm 2M}H_{laser}\ket{JKM}=\bigg[ \mp\frac{1}{4}\epsilon^2\bigg] \cdot \bigg[ \sqrt{(2J+1)(2J-1)}\bigg] [\alpha_{xx}-\alpha_{yy}]\\A_2(2J+2)^22M[6(J+M)(J-M)]^{1/2}\cdot \\ [4(J \mp K-2)(J \mp K-1)(J \mp K)(J \pm K+1)]^{1/2}
%\end{align*}

\subsection{$J'=J+2$}
\begin{align*}
  \bra{J+2KM}H_{laser}\ket{JKM}=\\
\bigg[-\frac{1}{4}\epsilon^2\bigg]\cdot \bigg[ \sqrt{(2J+1)(2J+5)}\bigg] \bigg[\frac{1}{3}[2\alpha_{zz}-\alpha_{xx}-\alpha_{yy}] 
\cdot A_2(2J+5)^2\cdot \\ 
[6(J-M+2)(J-M+1)(J+M+2)(J+M+1)]^{1/2} \cdot \\ 
[6(J-K+2)(J-K+1)(J+K+2)(J+K+1)]^{1/2}\bigg]
\end{align*}
%\begin{align*}
%  \bra{J+2K-2M}H_{laser}\ket{JKM}=\wigner{J}{2}{J+2}{-M}{0}{M}\wigner{J}{2}{J+2}{-K}{2}{K-2}=\\(-1)^{J+M}A_2(2J+5)[6(J-M+2)(J-M+1)(J+M+2)(J+M+1)]^{1/2}*\\(-1)^{J+K}A_2(2J+5)[(J-K+1)(J-K+2)(J-K+3)(J-K+4)]^{1/2}
%\end{align*}
%\begin{align*}
%  \bra{J+2K+2M}H_{laser}\ket{JKM}=\wigner{J}{2}{J+2}{-M}{0}{M}\wigner{J}{2}{J+2}{-K}{-2}{K+2}=\\(-1)^{J+M}A_2(2J+5)[6(J-M+2)(J-M+1)(J+M+2)(J+M+1)]^{1/2}*\\(-1)^{J+K}A_2(2J+5)[(J+K+1)(J+K+2)(J+K+3)(J+K+4)]^{1/2}
%\end{align*}
\begin{align*}
  \bra{J+2K\pm2M}H_{laser}\ket{JKM}= \bigg[ - \frac{1}{4}\epsilon^2 \bigg] \cdot \bigg[ \sqrt{(2J+1)(2J+5)}\bigg] [\alpha_{xx}-\alpha_{yy}] \cdot \\ A_2(2J+5)^2[6(J-M+2)(J-M+1)(J+M+2)(J+M+1)]^{1/2}\cdot \\ [(J\pm K+1)(J \pm K+2)(J \pm K+3)(J \pm K+4)]^{1/2}
\end{align*}

%\subsection{$J'=J-2$}
%\begin{align*}
%  \bra{J-2KM}H_{laser}\ket{JKM}= \\ \bigg[-\frac{1}{4}\epsilon^2\bigg]\cdot \bigg[ \sqrt{(2J+1)(2J-3)}\bigg]  \bigg[\frac{1}{3}[2\alpha_{zz}-\alpha_{xx}-\alpha_{yy}]\cdot \\  A_2(2J+1)^2[6(J+M)(J+M-1)(J-M)(J-M-1)]^{1/2}\cdot \\ [6(J+K)(J+K-1)(J-K)(J-K-1)]^{1/2}
%\end{align*}
%\begin{align*}
%  \bra{J-2K-2M}H_{laser}\ket{JKM}=\\(-1)^{J+M}A_2(2J+1)[6(J+M)(J+M-1)(J-M)(J-M-1)]^{1/2}*\\(-1)^{J+K}A_2(2J+1)[(J+K-3)(J+K-2)(J+K-1)(J+K)]^{1/2}
%\end{align*}
%\begin{align*}
%  \bra{J-2K+2M}H_{laser}\ket{JKM}=\\(-1)^{J+M}A_2(2J+1)[6(J+M)(J+M-1)(J-M)(J-M-1)]^{1/2}*\\(-1)^{J+K}A_2(2J+1)[(J-K-3)(J-K-2)(J-K-1)(J-K)]^{1/2}
%\end{align*}
%\begin{align*}
%  \bra{J-2K\pm 2M}H_{laser}\ket{JKM}=\bigg[ - \frac{1}{4}\epsilon^2 \bigg] \cdot \bigg[ \sqrt{(2J+1)(2J-3)}\bigg] [\alpha_{xx}-\alpha_{yy}] \cdot \\ A_2(2J+1)^2[6(J+M)(J+M-1)(J-M)(J-M-1)]^{1/2}\cdot \\ [(J \mp K-3)(J \mp K-2)(J \mp K-1)(J \mp K)]^{1/2}
%\end{align*}
\end{document}
%%% Local Variables: 
%%% mode: flyspell
%%% coding: utf-8
%%% TeX-master: t
%%% fill-column: 100
%%% TeX-auto-save: t
%%% TeX-parse-self: t
%%% End: 
